tests/lean/1467.lean
@@ -3,8 +3,8 @@ axiom H_f_g : ∀ n, f (g n) = n
 
 example (m : ℕ) : h m = h m :=
 begin
-definev n : ℕ := g m,
-assertv H : f n = m := begin dsimp, rw H_f_g end,
+pose n : ℕ := g m,
+note H : f n = m := begin dsimp, rw H_f_g end,
 subst H, -- Error here
 end
 
@@ -14,14 +14,14 @@ example (m : ℕ) : h m = h m :=
 begin
 define n : ℕ, -- add metavar
 exact g m,
-assertv H : f n = m := begin dsimp, rw H_f_g end,
+note H : f n = m := begin dsimp, rw H_f_g end,
 subst H, -- Error here
 end
 
 example (m : ℕ) : h m = h m :=
 begin
-definev n : ℕ := g m,
-assertv H : f n = m := begin dsimp, rw H_f_g end,
+pose n : ℕ := g m,
+note H : f n = m := begin dsimp, rw H_f_g end,
 subst m, -- Error here
 end
 
@@ -31,13 +31,13 @@ example (m : ℕ) : h m = h m :=
 begin
 define n : ℕ, -- add metavar
 exact g m,
-assertv H : f n = m := begin dsimp, rw H_f_g end,
+note H : f n = m := begin dsimp, rw H_f_g end,
 subst m, -- Error here
 end
 
 example (m p: ℕ) : h m = h m :=
 begin
-definev a : ℕ := g p,
-definev n : ℕ := g a,
+pose a : ℕ := g p,
+pose n : ℕ := g a,
 clear p -- Error here
 end
